code/experimental/curve25519/lemmas/Hacl.Spec.Curve25519.Field51.Lemmas.fst
@@ -874,3 +874,26 @@ let lemma_store_felem f =
   FStar.Math.Lemmas.multiple_modulo_lemma (v f4 % pow2 52) (pow2 12);
   logor_disjoint64 (f3 >>. 39ul) (f4 <<. 12ul) 12;
   lemma_store_felem0 f
+
+val lemma_cswap2_step:
+    bit:uint64{v bit <= 1}
+  -> p1:uint64
+  -> p2:uint64
+  -> Lemma (
+      let mask = u64 0 -. bit in
+      let dummy = mask &. (p1 ^. p2) in
+      let p1' = p1 ^. dummy in
+      let p2' = p2 ^. dummy in
+      if v bit = 1 then p1' == p2 /\ p2' == p1 else p1' == p1 /\ p2' == p2)
+let lemma_cswap2_step bit p1 p2 =
+  let mask = u64 0 -. bit in
+  assert (v bit == 0 ==> v mask == 0);
+  assert (v bit == 1 ==> v mask == pow2 64 - 1);
+  let dummy = mask &. (p1 ^. p2) in
+  assert (v bit == 1 ==> v dummy == v (p1 ^. p2));
+  assert (v bit == 0 ==> v dummy == 0);
+  let p1' = p1 ^. dummy in
+  uintv_extensionality dummy (if v bit = 1 then (p1 ^. p2) else u64 0);
+  logxor_lemma p1 p2;
+  let p2' = p2 ^. dummy in
+  logxor_lemma p2 p1
